<?xml version="1.0" encoding="UTF-8"?>
<rdf:RDF
   xmlns:dc="http://purl.org/dc/elements/1.1/"
   xmlns:rdf="http://www.w3.org/1999/02/22-rdf-syntax-ns#"
   xmlns:rdfs="http://www.w3.org/2000/01/rdf-schema#"
   xmlns:skos="http://www.w3.org/2004/02/skos/core#"
>
<rdf:Description rdf:about="https://vocabs.acdh.oeaw.ac.at/archeaccessrestrictions/Schema">
    <rdf:type rdf:resource="http://www.w3.org/2004/02/skos/core#ConceptScheme"/>
    <dc:title xml:lang="en">ARCHE access restrictions</dc:title>
    <dc:title xml:lang="de">ARCHE Zugriffsbeschränkungen</dc:title>
    <rdfs:label xml:lang="en">ARCHE access restrictions</rdfs:label>
    <rdfs:label xml:lang="de">ARCHE Zugriffsbeschränkungen</rdfs:label>
    <dc:description xml:lang="en">A list of access restriction types for ARCHE.</dc:description>
    <dc:description xml:lang="de">Eine Liste mit Typen von Zugriffsmöglichkeiten für ARCHE</dc:description>
    <dc:creator>Martina Trognitz</dc:creator>
    <dc:rights>https://creativecommons.org/licenses/by/4.0/</dc:rights>
    <dc:subject xml:lang="en">access restriction</dc:subject>
    <dc:subject xml:lang="de">Zugriffsbeschränkung</dc:subject>
    <dc:relation rdf:resource="https://arche.acdh.oeaw.ac.at/browser/"/>
    <dc:language>English</dc:language>
    <dc:language>German</dc:language>
    <dc:format>application/rdf+xml</dc:format>
    <skos:hasTopConcept rdf:resource="https://vocabs.acdh.oeaw.ac.at/archeaccessrestrictions/public"/>
    <skos:hasTopConcept rdf:resource="https://vocabs.acdh.oeaw.ac.at/archeaccessrestrictions/academic"/>
    <skos:hasTopConcept rdf:resource="https://vocabs.acdh.oeaw.ac.at/archeaccessrestrictions/restricted"/>
</rdf:Description>
  <rdf:Description rdf:about="https://vocabs.acdh.oeaw.ac.at/archeaccessrestrictions/public">
    <dc:source>CLARIN</dc:source>
    <skos:topConceptOf rdf:resource="https://vocabs.acdh.oeaw.ac.at/archeaccessrestrictions/Schema"/>
    <skos:prefLabel xml:lang="en">public</skos:prefLabel>
    <skos:prefLabel xml:lang="de">öffentlich</skos:prefLabel>
    <rdf:type rdf:resource="http://www.w3.org/2004/02/skos/core#Concept"/>
    <skos:definition xml:lang="en">Public resources are accessible without any further restrictions.</skos:definition>
    <skos:definition xml:lang="de">Öffentliche Ressourcen sind ohne Einschränkungen zugänglich.</skos:definition>
    <skos:inScheme rdf:resource="https://vocabs.acdh.oeaw.ac.at/archeaccessrestrictions/Schema"/>
  </rdf:Description>
  <rdf:Description rdf:about="https://vocabs.acdh.oeaw.ac.at/archeaccessrestrictions/academic">
    <dc:source>CLARIN</dc:source>
    <skos:topConceptOf rdf:resource="https://vocabs.acdh.oeaw.ac.at/archeaccessrestrictions/Schema"/>
    <skos:prefLabel xml:lang="en">academic</skos:prefLabel>
    <skos:prefLabel xml:lang="de">akademisch</skos:prefLabel>
    <rdf:type rdf:resource="http://www.w3.org/2004/02/skos/core#Concept"/>
    <skos:definition xml:lang="en">Academic access means that an affiliation with an academic institution is checked via Shibboleth login.</skos:definition>
    <skos:definition xml:lang="de">Akademischer Zugang bedeutet, dass die Zugehörigkeit an eine akademische Institution mittels Shibboleth-Login geprüft wird.</skos:definition>
    <skos:inScheme rdf:resource="https://vocabs.acdh.oeaw.ac.at/archeaccessrestrictions/Schema"/>
  </rdf:Description>
  <rdf:Description rdf:about="https://vocabs.acdh.oeaw.ac.at/archeaccessrestrictions/restricted">
    <dc:source>CLARIN</dc:source>
    <skos:topConceptOf rdf:resource="https://vocabs.acdh.oeaw.ac.at/archeaccessrestrictions/Schema"/>
    <skos:prefLabel xml:lang="en">restricted</skos:prefLabel>
    <skos:prefLabel xml:lang="de">eingeschränkt</skos:prefLabel>
    <rdf:type rdf:resource="http://www.w3.org/2004/02/skos/core#Concept"/>
    <skos:definition xml:lang="en">Restricted access requires registration and an a permission from the owner.</skos:definition>
    <skos:definition xml:lang="de">Beschränkter Zugang erfordert eine Registrierung und die Erlaubnis des Dateninhabers.</skos:definition>
    <skos:inScheme rdf:resource="https://vocabs.acdh.oeaw.ac.at/archeaccessrestrictions/Schema"/>
  </rdf:Description>
</rdf:RDF>